remove ideals from model, refactor

Core/model.v
@@ -27,63 +27,41 @@ Canonical Structure exn_eqType := EqType exn exn_eqMixin.
 Inductive ans (A : Type) : Type := Val of A | Exn of exn.
 Arguments Exn [A].
 
+(* A set of heaps *)
 Notation pre := (Pred heap).
+
+(* A set of (ans A * heap) *)
+(* This models the fact that programs can hang, returning nothing, *)
+(* or produce nondeterministic results (e.g. alloc). *)
 Notation post A := (ans A -> heap -> Prop).
-Definition spec G B := G -> pre * post B : Type.
+
+Definition spec G A := G -> pre * post A : Type.
 
 (********************************)
 (* Definition of the Hoare type *)
 (********************************)
 
-Definition defed (P : Pred heap) : Pred heap :=
-  [Pred i \In P | valid i].
-
-Lemma defed_leq h : defed h <== h.
-Proof. by move=>i []. Qed.
-
-Lemma defed_mono : monotone defed.
-Proof. by move=>h1 h2 H1 i [H2 V]; split=>//; apply: H1 H2. Qed.
-
-Notation ideald P := (ideal (defed P)).
-
-Definition relaxd P1 P2 (p : ideald P2) (pf : P2 <== P1) : ideald P1 :=
-  relax p (defed_mono pf).
-
-Lemma relaxd_refl P (p : ideald P) (pf : P <== P): relaxd p pf = p.
-Proof. by case: p=>p H; congr Ideal; apply: pf_irr. Qed.
-
-Lemma relaxd_trans P1 P2 P3 (p : ideald P1) (pf12 : P1 <== P2) (pf23 : P2 <== P3) (pf13 : P1 <== P3) :
-        relaxd (relaxd p pf12) pf23 = relaxd p pf13.
-Proof. by congr Ideal; apply: pf_irr. Qed.
-
 Section BasePrograms.
 Variables (P : pre) (A : Type).
 
-Lemma bound (p : ideald P) i : i \In id_val p -> i \In defed P.
-Proof. by case: p=>p; apply. Qed.
-
 (* we carve out the model out of the following base type *)
-Definition prog := ideald P -> ans A -> Pred heap.
+Definition prog := forall i, i \In P -> valid i -> post A.
 
-(* we take only progs with special properties *)
+(* we take only preconditions and progs with special properties *)
 (* which we define next *)
 
-(* coherence is continuity stated with *)
-(* directed sets instead of chains *)
-Definition coherent (e : prog) :=
-  forall p x m,
-    m \In e p x <-> exists i (pf : i \In id_val p),
-                    m \In e (single (bound pf)) x.
+(* safety monotonicity *)
+Definition safe_mono :=
+  forall i j, i \In P -> valid (i \+ j) -> i \+ j \In P.
 
 (* defined heaps map to defined heaps *)
-Definition def_strict (e : prog) := forall p x, Heap.Undef \Notin e p x.
+Definition def_strict (e : prog) := forall i p v x, Heap.Undef \Notin e i p v x.
 
-(* safety monotonicity + frame property *)
+(* frame property *)
 Definition frameable (e : prog) :=
-  forall i j (pf : i \In defed P) (V : valid (i \+ j)),
-    exists (pf' : i \+ j \In P),
-      forall y m, e (single (conj pf' V)) y m ->
-        exists h, m = h \+ j /\ valid (h \+ j) /\ e (single pf) y h.
+  forall i j (pf : i \In P) (V : valid (i \+ j)) (pf' : i \+ j \In P) y m,
+    e _ pf' V y m ->
+    exists h, [/\ m = h \+ j, valid (h \+ j) & e _ pf (validL V) y h].
 
 End BasePrograms.
 
@@ -93,21 +71,22 @@ Variable (A : Type).
 Structure ST := Prog {
   pre_of : pre;
   prog_of : prog pre_of A;
-  _ : coherent prog_of;
+  _ : safe_mono pre_of;
   _ : def_strict prog_of;
   _ : frameable prog_of}.
 
-Arguments prog_of : clear implicits.
-
-Lemma coh_st e : coherent (prog_of e).
+Lemma sfm_st e : safe_mono (pre_of e).
 Proof. by case: e. Qed.
 
-Arguments coh_st : clear implicits.
+Arguments sfm_st : clear implicits.
+
+Arguments prog_of : clear implicits.
 
 Lemma dstr_st e : def_strict (prog_of e).
 Proof. by case: e. Qed.
 
-Corollary dstr_valid e p x m : m \In prog_of e p x -> valid m.
+Corollary dstr_valid e i p v x m :
+            m \In prog_of e i p v x -> valid m.
 Proof. by case: m=>// /dstr_st. Qed.
 
 Arguments dstr_st : clear implicits.
@@ -117,67 +96,65 @@ Proof. by case: e. Qed.
 
 Arguments fr_st : clear implicits.
 
-Definition vrf i (c : ST) (Q : post A) :=
-  forall (V : valid i),
-    exists (pf : i \In pre_of c), forall y m,
-    prog_of c (single (conj pf V)) y m -> Q y m.
-
-Definition has_spec G (s : spec G A) (c : ST) :=
-  forall g i, (s g).1 i -> vrf i c (s g).2.
-
 (* poset structure on ST *)
 
 Definition st_leq e1 e2 :=
   exists pf : pre_of e2 <== pre_of e1,
-  forall p : ideald (pre_of e2),
-    prog_of e1 (relaxd p pf) <== prog_of e2 p.
+  forall i (p : i \In pre_of e2),
+    prog_of e1 _ (pf _ p) <== prog_of e2 _ p.
 
 Lemma st_refl e : st_leq e e.
-Proof. by exists (poset_refl _)=>p y m; rewrite relaxd_refl. Qed.
+Proof.
+exists (poset_refl _)=>i p V y m.
+by rewrite (pf_irr (poset_refl (pre_of e) i p) p).
+Qed.
 
 Lemma st_asym e1 e2 : st_leq e1 e2 -> st_leq e2 e1 -> e1 = e2.
 Proof.
-move: e1 e2=>[p1 e1 C1 D1 F1][p2 e2 C2 D2 F2]; rewrite /st_leq /=.
+move: e1 e2=>[p1 e1 S1 D1 F1][p2 e2 S2 D2 F2]; rewrite /st_leq /=.
 case=>E1 R1 [E2 R2].
 move: (poset_asym E1 E2)=>?; subst p2.
 have : e1 = e2.
-- apply: fext=>p; apply: fext=>y; apply: fext=>m.
-  move: (R2 p y m)=>{}R2; move: (R1 p y m)=>{}R1.
+- apply: fext=>i; apply: fext=>Hi; apply: fext=>Vi; apply: fext=>y; apply: fext=>m.
+  move: (R2 i Hi Vi y m)=>{}R2; move: (R1 i Hi Vi y m)=>{}R1.
   apply: pext; split.
-  - by move=>H1; apply: R1; rewrite relaxd_refl.
-  by move=>H2; apply: R2; rewrite relaxd_refl.
+  - by move=>H1; apply: R1; rewrite (pf_irr (E1 i Hi) Hi).
+  by move=>H2; apply: R2; rewrite (pf_irr (E2 i Hi) Hi).
 move=>?; subst e2.
 by congr Prog; apply: pf_irr.
 Qed.
 
 Lemma st_trans e1 e2 e3 : st_leq e1 e2 -> st_leq e2 e3 -> st_leq e1 e3.
 Proof.
-move: e1 e2 e3=>[p1 e1 C1 D1 F1][p2 e2 C2 D2 F2][p3 e3 C3 D3 F3].
+move: e1 e2 e3=>[p1 e1 S1 D1 F1][p2 e2 S2 D2 F2][p3 e3 S3 D3 F3].
 case=>/= E1 R1 [/= E2 R2]; rewrite /st_leq /=.
-have E3 := poset_trans E2 E1; exists E3=>p y m.
-set p' := relaxd p E2.
-move: (R1 p' y m)=>{}R1; move: (R2 p y m)=>{}R2.
+have E3 := poset_trans E2 E1; exists E3=>i P V y m.
+set P' := E2 i P.
+move: (R1 i P' V y m)=>{}R1; move: (R2 i P V y m)=>{}R2.
 move=>H1; apply/R2/R1.
-by rewrite relaxd_trans.
+by rewrite (pf_irr (E1 i P') (E3 i P)).
 Qed.
 
-(* a program that can always run but never returns (an endless loop) *)
-Definition prog_bot : prog PredT A :=
-  fun _ _ _ => False.
+(* bottom is a program that can always run but never returns (an endless loop) *)
 
-Lemma coherent_bot : coherent prog_bot.
-Proof. by move=>p y m; split=>//; case=>i []. Qed.
+Definition pre_bot : pre := top.
+
+Definition prog_bot : prog pre_bot A :=
+  fun _ _ _ _ _ => False.
+
+Lemma sfmono_bot : safe_mono pre_bot.
+Proof. by []. Qed.
 
 Lemma dstrict_bot : def_strict prog_bot.
 Proof. by move=>*. Qed.
 
 Lemma frame_bot : frameable prog_bot.
-Proof. by move=>i j [[] Vi] Vij; exists I. Qed.
+Proof. by []. Qed.
 
-Definition st_bot := Prog coherent_bot dstrict_bot frame_bot.
+Definition st_bot := Prog sfmono_bot dstrict_bot frame_bot.
 
 Lemma st_botP e : st_leq st_bot e.
-Proof. by case: e=>p e C D; exists (@pred_topP _ _)=>?; apply: botP. Qed.
+Proof. by case: e=>p e S D F; exists (@pred_topP _ _)=>???; apply: botP. Qed.
 
 Definition stPosetMixin := PosetMixin st_botP st_refl st_asym st_trans.
 Canonical stPoset := Eval hnf in Poset ST stPosetMixin.
@@ -193,67 +170,49 @@ Definition pre_sup_leq u e (pf : e \In u) : pre_sup u <== pre_of e :=
 
 (* union of postconditions *)
 Definition prog_sup (u : Pred ST) : prog (pre_sup u) A :=
-  fun p y m => exists e (pf : e \In u),
-    prog_of e (relaxd p (pre_sup_leq pf)) y m.
+  fun i P V y m => exists e (pf : e \In u),
+    prog_of e _ (pre_sup_leq pf P) V y m.
 
 Arguments prog_sup : clear implicits.
 
-Lemma prog_sup_coh u : coherent (prog_sup u).
+Lemma pre_sup_sfmono u : safe_mono (pre_sup u).
 Proof.
-move=>p y m; split.
-- case=>e [H1 H2]; have Cx := coh_st e.
-  case/Cx: H2=>i [pf1] M; exists i, pf1, e, H1.
-  apply/Cx; exists i.
-  set y' := id_val _; have J2 : i \In y' by [].
-  by exists J2; rewrite (pf_irr (bound J2) (bound pf1)).
-case=>i[pf][e][H1 H2]; have Cx := coh_st e.
-exists e, H1.
-case/Cx: H2=>i0 [E] M0; apply/Cx; exists i0.
-have J2 : i0 \In id_val (relaxd p (pre_sup_leq H1)).
-- by rewrite -E /=.
-by exists J2; rewrite (pf_irr (bound J2) (bound E)).
+move=>i j Pi Vij e He.
+by apply: sfm_st=>//; apply: Pi.
 Qed.
 
 Lemma prog_sup_dstrict u : def_strict (prog_sup u).
-Proof. by move=>p y; case; case=>p0 e C D F [H1] /D. Qed.
+Proof. by move=>i P V y; case; case=>p e S D F [H1] /D. Qed.
 
 Lemma prog_sup_frame u : frameable (prog_sup u).
 Proof.
-move=>i j [Hi Vi] Vij.
-have J : i \+ j \In pre_sup u.
-- move=>e He; move: (Hi _ He)=>{}Hi.
-  by case: (fr_st e _ _ (conj Hi Vi) Vij).
-exists J=>y m [e][He]Pe.
-move: (Hi e He)=>Hi'.
-case: (fr_st e _ _ (conj Hi' Vi) Vij)=>pf P; move: Pe.
-rewrite (_ : relaxd (single (conj J Vij)) (pre_sup_leq He) = single (conj pf Vij));
-  last by congr Ideal; apply: pf_irr.
-case/P=>h' [E][V']P'.
-exists h'; do!split=>//; exists e, He.
-rewrite (_ : relaxd (single (conj Hi Vi)) (pre_sup_leq He) = single (conj Hi' Vi)) //.
-by congr Ideal; apply: pf_irr.
+move=>i j Pi Vij Pij y m [e][He]Pe.
+have Pi' := Pi e He; have Pij' := Pij e He.
+have P := fr_st _ _ _ Pi' Vij Pij' y m.
+move: Pe; rewrite (pf_irr (pre_sup_leq He Pij) Pij').
+case/P=>h [{m P}-> Vhj Ph].
+exists h; split=>//; exists e, He.
+by rewrite (pf_irr (pre_sup_leq He Pi) Pi').
 Qed.
 
-Definition st_sup u := Prog (@prog_sup_coh u) (@prog_sup_dstrict u) (@prog_sup_frame u).
+Definition st_sup u := Prog (@pre_sup_sfmono u) (@prog_sup_dstrict u) (@prog_sup_frame u).
 
 Lemma st_supP u e : e \In u -> e <== st_sup u.
 Proof.
-case: e=>p e' C D F R.
+case: e=>p e' S D F R.
 exists (pre_sup_leq R)=>/=p0 y m H.
-by exists (Prog C D F), R.
+by exists (Prog S D F), R.
 Qed.
 
 Lemma st_supM u e :
   (forall e1, e1 \In u -> e1 <== e) -> st_sup u <== e.
 Proof.
-case: e=>p e C D F R.
+case: e=>p e S D F R.
 have J : p <== pre_sup u.
 - by move=>/= x Px e' pf; case: (R _ pf)=>/= + _; apply.
-exists J=>p0 y m [e0][pf H1]; have Cx := coh_st e0.
-case: (R _ pf)=>/= Hx; apply=>//.
-case/Cx: H1=>i [pf1 M1]; apply/Cx; exists i.
-have J2 : i \In id_val (relaxd p0 Hx) by exact: pf1.
-by exists J2; rewrite (pf_irr (bound J2) (bound pf1)).
+exists J=>i P V y m [e0][H0 Hm].
+case: (R _ H0)=>/= Hx; apply.
+by rewrite (pf_irr (Hx i P) (pre_sup_leq H0 (J i P))).
 Qed.
 
 Definition stLatticeMixin := LatticeMixin st_supP st_supM.
@@ -262,15 +221,26 @@ Canonical stLattice := Lattice ST stLatticeMixin.
 End STDef.
 
 Arguments prog_of [A].
-Arguments coh_st [A].
+Arguments sfm_st [A].
 Arguments dstr_st [A].
+Arguments fr_st [A].
 
 Section STspecDef.
 Variables (G A : Type) (s : spec G A).
 
+(* predicate transformer *)
+
+Definition vrf i (e : ST A) (Q : post A) :=
+  forall (V : valid i),
+    exists (pf : i \In pre_of e), forall y m,
+      prog_of e _ pf V y m -> Q y m.
+
+Definition has_spec (e : ST A) :=
+  forall g i, (s g).1 i -> vrf i e (s g).2.
+
 Structure STspec := STprog {
   model : ST A;
-  _ : model \In has_spec s}.
+  _ : model \In has_spec}.
 
 Lemma modelE e1 e2 : e1 = e2 <-> model e1 = model e2.
 Proof.
@@ -298,12 +268,8 @@ move: e1 e2 e3=>[e1 H1][e2 H2][e3 H3].
 by apply: poset_trans.
 Qed.
 
-Lemma st_bot_has_spec : @st_bot A \In has_spec s.
-Proof.
-move=>g i H V /=.
-have J: i \In PredT by [].
-by exists J.
-Qed.
+Lemma st_bot_has_spec : @st_bot A \In has_spec.
+Proof. by move=>g i H V /=; exists I. Qed.
 
 Definition stsp_bot := STprog st_bot_has_spec.
 
@@ -318,15 +284,15 @@ Canonical stspPoset := Eval hnf in Poset STspec stspPosetMixin.
 Definition st_sup' (u : Pred STspec) : ST A :=
   sup [Pred p | exists e, p = model e /\ e \In u].
 
-Lemma st_sup_has_spec' u : st_sup' u \In has_spec s.
+Lemma st_sup_has_spec' u : st_sup' u \In has_spec.
 Proof.
 move=>g i p Vi.
 have J : i \In pre_of (st_sup' u).
 - by move=>_ [e][->]; case: e=>e P; case: (P _ _ p Vi).
 exists J=>y m /= [e][[[e1 P]]][/= E He1] H; subst e1.
-set I' := (X in prog_of e X) in H.
 case: (P _ _ p Vi)=>Hi; apply.
-by rewrite (_ : single (conj Hi Vi) = I') //; congr Ideal; apply: pf_irr.
+set I' := (X in prog_of e i X) in H.
+by rewrite (pf_irr Hi I').
 Qed.
 
 Definition stsp_sup u := STprog (@st_sup_has_spec' u).
@@ -367,7 +333,7 @@ move=>x y H; apply: sup_mono=>fz; case=>z [Hz {fz}->].
 by exists z; split=>//; apply/poset_trans/H.
 Qed.
 
-Definition ffix : tp := tarski_lfp f'.
+Definition Fix : tp := tarski_lfp f'.
 
 End Fix.
 
@@ -387,10 +353,11 @@ Lemma vrf_frame A i j (e : ST A) (Q : post A) :
         vrf (i \+ j) e Q.
 Proof.
 move=>H Vij; have Vi := validL Vij; case: (H Vi)=>Hi {}H.
-case: (fr_st (conj Hi Vi) Vij)=>pf P.
-exists pf=>y m.
-case/P=>h [{m}->][Vhj {}P].
-by apply: H.
+have Hij := sfm_st _ _ _ Hi Vij.
+exists Hij=>y m.
+case/(fr_st _ _ _ Hi Vij Hij)=>h [{m}-> Vhj P].
+apply: H=>//.
+by rewrite (pf_irr Vi (validL Vij)).
 Qed.
 
 Lemma frame_star A i (e : ST A) (Q : post A) (r : Pred heap) :
@@ -415,64 +382,52 @@ Qed.
 Section Return.
 Variables (A : Type) (x : A).
 
-Definition ret_pre : pre := PredT.
+Definition ret_pre : pre := top.
 
 Definition ret_prog : prog ret_pre A :=
-  fun p y m =>
-    m \In id_val p /\ y = Val x.
+  fun i _ _ y m =>
+    m = i /\ y = Val x.
 
-Lemma ret_coherent : coherent ret_prog.
-Proof.
-move=>p y m; split; first by case=>H {y}->; exists m, H.
-by case=>i [Hi][{m}<-{y}->].
-Qed.
+Lemma ret_sfmono : safe_mono ret_pre.
+Proof. by []. Qed.
 
 Lemma ret_dstrict : def_strict ret_prog.
-Proof. by case=>p H y /= []; case/H. Qed.
+Proof. by move=>i [] V _ /= [E _]; rewrite -E in V. Qed.
 
 Lemma ret_frame : frameable ret_prog.
-Proof.
-move=>i j [[] Hv] Vij.
-by exists I=>_ _ [<- ->]; exists i.
-Qed.
+Proof. by move=>i j [Vij []] _ _ [-> ->]; exists i. Qed.
 
-Definition ret := Prog ret_coherent ret_dstrict ret_frame.
+Definition ret := Prog ret_sfmono ret_dstrict ret_frame.
 
 Lemma vrf_ret (Q : post A) i :
         Q (Val x) i -> vrf i ret Q.
-Proof. by move=>Hi V; exists I=>_ _ [<- ->]. Qed.
+Proof. by move=>H V; exists I=>_ _ [->->]. Qed.
 
 End Return.
 
 Section Throw.
 Variables (A : Type) (e : exn).
 
-Definition throw_pre : pre := PredT.
+Definition throw_pre : pre := top.
 
 Definition throw_prog : prog throw_pre A :=
-  fun p y m =>
-    m \In id_val p /\ y = @Exn A e.
+  fun i _ _ y m =>
+    m = i /\ y = @Exn A e.
 
-Lemma throw_coherent : coherent throw_prog.
-Proof.
-move=>p y m; split; first by case=>H {y}->; exists m, H.
-by case=>i [Hi][{m}<-{y}->].
-Qed.
+Lemma throw_sfmono : safe_mono throw_pre.
+Proof. by []. Qed.
 
 Lemma throw_dstrict : def_strict throw_prog.
-Proof. by case=>p H y /= []; case/H. Qed.
+Proof. by move=>i [] V _ /= [E _]; rewrite -E in V. Qed.
 
 Lemma throw_frame : frameable throw_prog.
-Proof.
-move=>i j [[] Hv] Vij.
-by exists I=>_ _ [<- ->]; exists i.
-Qed.
+Proof. by move=>i j [Vij []] _ _ [-> ->]; exists i. Qed.
 
-Definition throw := Prog throw_coherent throw_dstrict throw_frame.
+Definition throw := Prog throw_sfmono throw_dstrict throw_frame.
 
 Lemma vrf_throw (Q : post A) i :
         Q (Exn e) i -> vrf i throw Q.
-Proof. by move=>Hi V; exists I=>_ _ [<- ->]. Qed.
+Proof. by move=>H V; exists I=>_ _ [->->]. Qed.
 
 End Throw.
 
@@ -481,63 +436,58 @@ Variables (A B : Type).
 Variables (e1 : ST A) (e2 : A -> ST B).
 
 Definition bind_pre : pre :=
-  fun i => exists pf : i \In defed (pre_of e1),
-    forall x m, prog_of e1 (single pf) (Val x) m -> pre_of (e2 x) m.
+  fun i =>
+    exists (Pi : i \In pre_of e1) (Vi : valid i),
+      forall x m, prog_of e1 i Pi Vi (Val x) m -> pre_of (e2 x) m.
+
+Definition bind_pre_proj i : i \In bind_pre -> i \In pre_of e1 :=
+  fun '(ex_intro e _) => e.
 
 Definition bind_prog : prog bind_pre B :=
-  fun p y m =>
-    exists i x h, i \In id_val p /\
-      exists pf : i \In defed (pre_of e1),
-        h \In prog_of e1 (single pf) x /\
-        match x with
-        | Val x' => exists pf' : h \In defed (pre_of (e2 x')),
-                      m \In prog_of (e2 x') (single pf') y
-        | Exn e => y = Exn e /\ m = h
-        end.
+  fun i P V y m =>
+    exists x h (Ph : h \In prog_of e1 i (bind_pre_proj P) V x),
+      match x with
+      | Val x' => exists Ph' : h \In pre_of (e2 x'),
+                    m \In prog_of (e2 x') h Ph' (dstr_valid Ph) y
+      | Exn e => y = Exn e /\ m = h
+      end.
 
-Lemma bind_coherent : coherent bind_prog.
+Lemma bind_sfmono : safe_mono bind_pre.
 Proof.
-move=>p y m; split=>/=.
-- case=>i [x][h][H1][H2]H3.
-  by exists i, H1, i, x, h; split=>//; exists H2.
-case=>i [/= H1][_][x][h][<-][H2 H3].
-by exists i, x, h; split=>//=; exists H2.
+move=>i j [Pi][Vi]P Vij.
+have Pij := sfm_st _ _ _ Pi Vij.
+exists Pij, Vij=>x m.
+case/(fr_st _ _ _ Pi Vij Pij)=>h [{m}-> Vhj].
+rewrite (pf_irr (validL Vij) Vi)=>/P Ph.
+by apply: sfm_st=>//; apply: (validL Vhj).
 Qed.
 
 Lemma bind_dstrict : def_strict bind_prog.
 Proof.
-move=>p y [i][x][h][H1][H2][].
-case: x=>[x'|e] H3.
-- by case=>H4 /dstr_st.
-by case=>_; move: H3=>/[swap]<- /dstr_st.
+move=>i [P1][Vi P] Vi' y[x][h][/=].
+case: x=>[x|e]Ph.
+- by case=>Ph' /dstr_st.
+by case=>_; move: Ph=>/[swap]<- /dstr_st.
 Qed.
 
 Lemma bind_frame : frameable bind_prog.
 Proof.
-move=>i j [[Hi P] Hv] Vij; case: (fr_st Hi Vij)=>pf H.
-have Hij : i \+ j \In bind_pre.
-- exists (conj pf Vij)=>x _ /H [h][->][Vhj] /P {}P.
-  have Hh : h \In defed (pre_of (e2 x)) by split=>//; apply: (validL Vhj).
-  by case: (fr_st Hh Vhj).
-exists Hij=>y m; case=>_[x][h][<-][{}Hij][Hh].
-rewrite (pf_irr (conj pf Vij) Hij) in H.
-case: x Hh=>[x|e] Hh.
-- case=>Hh' Pm.
-  case/H: Hh=>h1 [Eh][Vh]P1.
-  rewrite Eh in Hh' Pm; move: (P _ _ P1)=>Hh1.
-  have J1 : h1 \In defed (pre_of (e2 x)) by split=>//; apply: (validL Vh).
-  case: (fr_st J1 Vh)=>pf1.
-  rewrite (_ : single (conj pf1 Vh) = single Hh'); last by congr Ideal; apply: pf_irr.
-  case/(_ _ _ Pm)=>h2[Em][Vm]Ph2.
-  exists h2; do!split=>//; exists i, (Val x), h1; split=>//.
-  by exists Hi; split=>//; exists J1.
+move=>i j [Pi [Vi P]] Vij [Pij _] y m [x][h][/=].
+move: (fr_st _ _ _ Pi Vij Pij)=>H.
+case: x=>[x|e] Ph.
+- case=>Ph'.
+  case: (H _ _ Ph)=>h1[Eh V1 Ph1]; subst h.
+  rewrite (pf_irr (validL Vij) Vi) in Ph1 *; move: (P _ _  Ph1)=> P21.
+  rewrite (pf_irr (dstr_valid Ph) V1).
+  case/(fr_st _ _ _ P21 V1 Ph')=>h2[Em Vm Ph2].
+  exists h2; split=>//; exists (Val x), h1, Ph1, P21.
+  by rewrite (pf_irr (dstr_valid Ph1) (validL V1)).
 case=>->->.
-case/H: Hh=>h1[Eh][Vh]Ph1.
-exists h1; do!split=>//; exists i, (Exn e), h1; split=>//.
-by exists Hi.
+case/H: Ph=>h1[Eh Vh Ph1].
+by exists h1; split=>//; exists (Exn e), h1, Ph1.
 Qed.
 
-Definition bind := Prog bind_coherent bind_dstrict bind_frame.
+Definition bind := Prog bind_sfmono bind_dstrict bind_frame.
 
 Lemma vrf_bind (Q : post B) i :
         vrf i e1 (fun x m => match x with
@@ -548,18 +498,15 @@ Lemma vrf_bind (Q : post B) i :
 Proof.
 move=>H Vi; case: (H Vi)=>Hi {}H /=.
 have Hi' : i \In bind_pre.
-- exists (conj Hi Vi)=>x m Pm.
+- exists Hi, Vi=>x m Pm.
   by case: (H _ _ Pm (dstr_valid Pm)).
-exists Hi'=>y j /= [_][x][m][<-][{}Hi'][Pm]C.
-rewrite (_ : single (conj Hi Vi) = single Hi') in H;
-  last by congr Ideal; apply: pf_irr.
-have Vm := dstr_valid Pm.
-case: x Pm C=>[x|e] Pm.
-- case=>Hm2 Pj.
-  move: (H _ _ Pm); case/(_ Vm)=>Hm; apply.
-  rewrite (_ : single (conj Hm Vm) = single Hm2) //.
-  by congr Ideal; apply: pf_irr.
-by case=>->->; apply: (H _ _ Pm).
+exists Hi'=>y j /= [x][m][Pm]C.
+rewrite (pf_irr Hi (bind_pre_proj Hi')) in H.
+case: x Pm C=>[x|e] Pm; move: (H _ _ Pm)=>{}H.
+- case=>Pm2 Pj.
+  case: (H (dstr_valid Pm))=>Pm2'; apply.
+  by rewrite (pf_irr Pm2' Pm2).
+by case=>->->.
 Qed.
 
 End Bind.
@@ -570,77 +517,67 @@ Variables (A B : Type).
 Variables (e : ST A) (e1 : A -> ST B) (e2 : exn -> ST B).
 
 Definition try_pre : pre :=
-  fun i => exists pf : i \In defed (pre_of e),
-             (forall y m, prog_of e (single pf) (Val y) m -> pre_of (e1 y) m) /\
-              forall ex m, prog_of e (single pf) (Exn ex) m -> pre_of (e2 ex) m.
+  fun i =>
+    exists (Pi : i \In pre_of e) (Vi : valid i),
+      (forall y  m, prog_of e i Pi Vi (Val y)  m -> pre_of (e1 y)  m) /\
+       forall ex m, prog_of e i Pi Vi (Exn ex) m -> pre_of (e2 ex) m.
+
+Definition try_pre_proj i : i \In try_pre -> i \In pre_of e :=
+  fun '(ex_intro e _) => e.
 
 Definition try_prog : prog try_pre B :=
-  fun p y m =>
-    exists i x h, i \In id_val p /\
-      exists pf : i \In defed (pre_of e),
-        h \In prog_of e (single pf) x /\
-        match x with
-        | Val x' => exists pf' : h \In defed (pre_of (e1 x')),
-                      m \In prog_of (e1 x') (single pf') y
-        | Exn ex => exists pf' : h \In defed (pre_of (e2 ex)),
-                      m \In prog_of (e2 ex) (single pf') y
-        end.
+  fun i P V y m =>
+    exists x h (Ph : h \In prog_of e i (try_pre_proj P) V x),
+      match x with
+      | Val x' => exists (Ph' : h \In pre_of (e1 x')),
+                    m \In prog_of (e1 x') h Ph' (dstr_valid Ph) y
+      | Exn ex => exists (Ph' : h \In pre_of (e2 ex)),
+                    m \In prog_of (e2 ex) h Ph' (dstr_valid Ph) y
+      end.
 
-Lemma try_coherent : coherent try_prog.
+Lemma try_sfmono : safe_mono try_pre.
 Proof.
-move=>p y m; split.
-- case=>i [x][h][/= H1][H2] H3.
-  by exists i, H1, i, x, h; split=>//; exists H2.
-case=>i [/= H1][_][x][h][<-][H2 H3].
-by exists i, x, h; split=>//; exists H2.
+move=>i j [Pi [Vi][E1 E2]] Vij.
+have Pij := sfm_st _ _ _ Pi Vij.
+exists Pij, Vij; split.
+- move=>y m.
+  case/(fr_st _ _ _ Pi Vij Pij)=>h [{m}-> Vhj].
+  rewrite (pf_irr (validL Vij) Vi)=>/E1 Ph.
+  by apply: sfm_st=>//; apply: (validL Vhj).
+move=>ex m.
+case/(fr_st _ _ _ Pi Vij Pij)=>h [{m}-> Vhj].
+rewrite (pf_irr (validL Vij) Vi)=>/E2 Ph.
+by apply: sfm_st=>//; apply: (validL Vhj).
 Qed.
 
 Lemma try_dstrict : def_strict try_prog.
 Proof.
-move=>p y [i][x][h][H1][H2][].
-by case: x=>[x'|e'] H3; case=>H4 /dstr_st.
+move=>i [Pi [Vi][E1 E2]] Vi' y[x][h][/=].
+by case: x=>[x|ex] Eh; case=>Ph /dstr_st.
 Qed.
 
 Lemma try_frame : frameable try_prog.
 Proof.
-move=>i j [[Hi [P1 P2]] Vi] Vij; case: (fr_st Hi Vij)=>pf H.
-have J : i \+ j \In try_pre.
-- exists (conj pf Vij); split.
-  - move=>x _ /H [h][->][Vhj] /P1 {}P1.
-    have J' : h \In defed (pre_of (e1 x)) by split=>//; apply: (validL Vhj).
-    by case: (fr_st J' Vhj).
-  move=>ex _ /H [h][->][Vhj] /P2 {}P2.
-  have J' : h \In defed (pre_of (e2 ex)) by split=>//; apply: (validL Vhj).
-  by case: (fr_st J' Vhj).
-exists J=>y m; case=>_[x][h1][<-][H0][H1].
-rewrite (_ : single (conj pf Vij) = single H0) in H;
-  last by congr Ideal; apply: pf_irr.
-case: x H1=>[x|ex] H1.
-- case=>H1' Po.
-  case: (H _ _ H1)=>h'[E'][V']P'.
-  rewrite E' in H1' Po; move: (P1 _ _ P')=>H1''.
-  have J' : h' \In defed (pre_of (e1 x)) by split=>//; apply: (validL V').
-  case: (fr_st J' V')=>pf2.
-  rewrite (_ : single (conj pf2 V') = single H1');
-    last by congr Ideal; apply: pf_irr.
-  case/(_ _ _ Po)=>h''[E''][V'']P''.
-  exists h''; do!split=>//.
-  exists i, (Val x), h'=>/=; split=>//.
-  by exists Hi; split=>//; exists J'.
-case=>H1' Po.
-case: (H _ _ H1)=>h'[E'][V']P'.
-rewrite E' in H1' Po; move: (P2 _ _ P')=>H1''.
-have J' : h' \In defed (pre_of (e2 ex)) by split=>//; apply: (validL V').
-case: (fr_st J' V')=>pf2.
-rewrite (_ : single (conj pf2 V') = single H1');
-  last by congr Ideal; apply: pf_irr.
-case/(_ _ _ Po)=>h''[E''][V'']P''.
-exists h''; do!split=>//.
-exists i, (Exn ex), h'=>/=; split=>//.
-by exists Hi; split=>//; exists J'.
+move=>i j [Pi [Vi][E1 E2]] Vij [Pij _] y m [x][h][/=].
+move: (fr_st _ _ _ Pi Vij Pij)=>H.
+case: x=>[x|ex] Ph.
+- case=>Ph'.
+  case: (H _ _ Ph)=>h1[Eh V1 Ph1]; subst h.
+  rewrite (pf_irr (validL Vij) Vi) in Ph1 *; move: (E1 _ _  Ph1)=>P21.
+  rewrite (pf_irr (dstr_valid Ph) V1).
+  case/(fr_st _ _ _ P21 V1 Ph')=>h2[Em Vm Ph2].
+  exists h2; split=>//; exists (Val x), h1, Ph1, P21.
+  by rewrite (pf_irr (dstr_valid Ph1) (validL V1)).
+case=>Ph'.
+case: (H _ _ Ph)=>h1[Eh V1 Ph1]; subst h.
+rewrite (pf_irr (validL Vij) Vi) in Ph1 *; move: (E2 _ _  Ph1)=> P21.
+rewrite (pf_irr (dstr_valid Ph) V1).
+case/(fr_st _ _ _ P21 V1 Ph')=>h2[Em Vm Ph2].
+exists h2; split=>//; exists (Exn ex), h1, Ph1, P21.
+by rewrite (pf_irr (dstr_valid Ph1) (validL V1)).
 Qed.
 
-Definition try := Prog try_coherent try_dstrict try_frame.
+Definition try := Prog try_sfmono try_dstrict try_frame.
 
 Lemma vrf_try (Q : post B) i :
         vrf i e (fun x m => match x with
@@ -649,23 +586,15 @@ Lemma vrf_try (Q : post B) i :
                  end) ->
         vrf i try Q.
 Proof.
-move=>H Vi; case: (H Vi)=>pf P /=.
+move=>H Vi; case: (H Vi)=>pf {}H /=.
 have J : i \In try_pre.
-- exists (conj pf Vi); split=>x m Pm;
-  by case: (P _ _ Pm (dstr_valid Pm)).
-exists J=>y j /= [_][x][m][<-][pf'][Pm]F.
-rewrite (_ : single (conj pf Vi) = single pf') in P;
-  last by congr Ideal; apply: pf_irr.
-have Vm := dstr_valid Pm.
-case: x Pm F=>[x|ex] Pm.
-- case=>Hm Hj.
-  case: (P _ _ Pm Vm)=>pf''; apply.
-  rewrite (_ : single (conj pf'' Vm) = single Hm) //.
-  by congr Ideal; apply: pf_irr.
-case=>Hm Hj.
-case: (P _ _ Pm Vm)=>pf''; apply.
-rewrite (_ : single (conj pf'' Vm) = single Hm) //.
-by congr Ideal; apply: pf_irr.
+- exists pf, Vi; split=>x m Pm;
+  by case: (H _ _ Pm (dstr_valid Pm)).
+exists J=>y j /= [x][m][Pm]F.
+rewrite (pf_irr pf (try_pre_proj J)) in H.
+case: x Pm F=>[x|ex] Pm [Hm Hj];
+case: (H _ _ Pm (dstr_valid Pm))=>pf''; apply;
+by rewrite (pf_irr pf'' Hm).
 Qed.
 
 End Try.
@@ -680,32 +609,27 @@ Definition read_pre : pre :=
   fun i => x \in dom i /\ exists v : A, find x i = Some (idyn v).
 
 Definition read_prog : prog read_pre A :=
-  fun p y m =>
-    m \In id_val p /\ exists w, y = Val w /\ find x m = Some (idyn w).
+  fun i _ _ y m =>
+    exists w, [/\ m = i, y = Val w & find x m = Some (idyn w)].
 
-Lemma read_coherent : coherent read_prog.
+Lemma read_sfmono : safe_mono read_pre.
 Proof.
-move=>p v m; split; last first.
-- by case=>i [H1][<-][w][->]; split=>//; exists w.
-case=>H1 [w][->] H2.
-by exists m, H1; split=>//; exists w.
+move=>i j [Hx [v E]] Vij; split.
+- by rewrite domUn inE Vij Hx.
+by exists v; rewrite findUnL // Hx.
 Qed.
 
 Lemma read_dstrict : def_strict read_prog.
-Proof. by case=>p H y []; case/H. Qed.
+Proof. by move=>i _ Vi _ [_ [E _ _]]; rewrite -E in Vi. Qed.
 
 Lemma read_frame : frameable read_prog.
 Proof.
-move=>i j [[Hx][v E] Vi] Vij.
-have J : i \+ j \In read_pre.
-- split; first by rewrite domUn inE Vij Hx.
-  by exists v; rewrite findUnL // Hx.
-exists J=>y m [/= <-][w][->]H.
-exists i; do!split=>//; exists w; split=>//.
+move=>i j [Hx [v E]] Vij _ _ _ [w [-> -> H]].
+exists i; split=>//; exists w; split=>{v E}//.
 by rewrite findUnL // Hx in H.
 Qed.
 
-Definition read := Prog read_coherent read_dstrict read_frame.
+Definition read := Prog read_sfmono read_dstrict read_frame.
 
 Lemma vrf_read (Q : post A) (v : A) j :
        (valid (x :-> v \+ j) -> Q (Val v) (x :-> v \+ j)) ->
@@ -715,7 +639,7 @@ move=>H Vi /=.
 have J : x :-> v \+ j \In read_pre.
 - split; first by rewrite domPtUnE.
   by exists v; rewrite findPtUn.
-exists J=>_ _ [<-][w][->].
+exists J=>_ _ [w [->->]].
 rewrite findPtUn //; case=>/inj_pair2 {w}<-.
 by apply: H.
 Qed.
@@ -732,35 +656,32 @@ Definition write_pre : pre :=
   fun i => x \in dom i.
 
 Definition write_prog : prog write_pre unit :=
-  fun p y m =>
-    exists i, [/\ y = Val tt, m = upd x (idyn v) i,
-                  i \In id_val p & x \in dom i].
+  fun i _ _ y m =>
+    [/\ y = Val tt, m = upd x (idyn v) i & x \in dom i].
 
-Lemma write_coherent : coherent write_prog.
+Lemma write_sfmono : safe_mono write_pre.
 Proof.
-move=>p y m; split.
-- by case=>i [{y}-> {m}-> Hi Hx]; exists i, Hi, i.
-by case=>i [Hi][_][{y}-> {m}-> <- Hx]; exists i.
+move=>i j; rewrite /write_pre -!toPredE /= => Hx Vij.
+by rewrite domUn inE Vij Hx.
 Qed.
 
 Lemma write_dstrict : def_strict write_prog.
 Proof.
-case=>p H y [i] /= [_ E Hi Hx].
-suff L: valid (upd x (idyn v) i) by rewrite -E in L.
+move=>i Hx _ _ [_ E _]; rewrite /write_pre -toPredE /= in Hx.
+suff {E}: valid (upd x (idyn v) i) by rewrite -E.
 by rewrite validU (dom_cond Hx) (dom_valid Hx).
 Qed.
 
 Lemma write_frame : frameable write_prog.
 Proof.
-move=>i j [Hi Vi] Vij.
-have J : i \+ j \In write_pre.
-- by rewrite /write_pre -toPredE /= domUn inE Vij Hi.
-exists J=>_ _ [_][->-> <- _]; exists (upd x (idyn v) i).
-rewrite updUnL Hi validUUn //; do!split=>//.
-by exists i.
+move=>i j Hx Vij _ _ _ [-> -> _].
+exists (upd x (idyn v) i); split=>//;
+rewrite /write_pre -toPredE /= in Hx.
+- by rewrite updUnL Hx.
+by rewrite validUUn.
 Qed.
 
-Definition write := Prog write_coherent write_dstrict write_frame.
+Definition write := Prog write_sfmono write_dstrict write_frame.
 
 Lemma vrf_write (Q : post unit) j B (u : B) :
         (valid (x :-> v \+ j) -> Q (Val tt) (x :-> v \+ j)) ->
@@ -769,7 +690,7 @@ Proof.
 move=>H Vi /=.
 have J : x :-> u \+ j \In write_pre.
 - by rewrite /write_pre -toPredE /= domPtUnE.
-exists J=>_ _ [_][->-> <- _].
+exists J=>_ _ [->-> _].
 rewrite updPtUn; apply: H.
 by rewrite (@validPtUnE _ _ _ _ (idyn u)).
 Qed.
@@ -782,49 +703,42 @@ Variables (A : Type) (v : A).
 
 Local Notation idyn v := (@dyn _ id _ v).
 
-Definition alloc_pre : pre := PredT.
+Definition alloc_pre : pre := top.
 
 Definition alloc_prog : prog alloc_pre ptr :=
-  fun p y m =>
-    exists i l, [/\ y = Val l, m = l :-> v \+ i, i \In id_val p,
-                    l != null & l \notin dom i].
+  fun i _ _ y m =>
+    exists l, [/\ y = Val l, m = l :-> v \+ i,
+                  l != null & l \notin dom i].
 
-Lemma alloc_coherent : coherent alloc_prog.
-Proof.
-move=>p x m; split.
-- case=>i[l][{x}-> {m}-> Hi Hl1 Hl2].
-  by exists i, Hi, i, l.
-case=>i[Hi][_][l][{x}-> {m}-> <- Hl1 Hl2].
-by exists i, l.
-Qed.
+Lemma alloc_sfmono : safe_mono alloc_pre.
+Proof. by []. Qed.
 
 Lemma alloc_dstrict : def_strict alloc_prog.
 Proof.
-case=>p H _ [/= i][l][_ Hu Hi Hl1 Hl2]; case/H: Hi=>_ {H}Vi.
-suff {Hu}: valid (l :-> v \+ i) by rewrite -Hu.
+move=>i [] Vi _ [l][_ E Hl Hl2].
+suff {E}: valid (l :-> v \+ i) by rewrite -E.
 by rewrite validPtUn; apply/and3P.
 Qed.
 
 Lemma alloc_frame : frameable alloc_prog.
 Proof.
-move=>i j [[]] Vi Vij.
-exists I=>_ _ [_][x][-> -> <- Hx1 Hx2].
-exists (x :-> v \+ i); rewrite -joinA; do!split=>//.
-- rewrite validUnAE validPt domPtK Hx1 Vij /= all_predC.
+move=>i j [] Vij [] _ _ [l][->-> Hl Hl2].
+exists (l :-> v \+ i); rewrite -joinA; split=>//.
+- rewrite validUnAE validPt domPtK Hl Vij /= all_predC.
   apply/hasP=>[[y Hy]]; rewrite !inE=>/eqP E.
-  by move: Hy Hx2; rewrite E=>->.
-exists i, x; split=>//.
-by apply/dom_NNL/Hx2.
+  by move: Hy Hl2; rewrite E=>->.
+exists l; split=>//.
+by apply/dom_NNL/Hl2.
 Qed.
 
-Definition alloc := Prog alloc_coherent alloc_dstrict alloc_frame.
+Definition alloc := Prog alloc_sfmono alloc_dstrict alloc_frame.
 
 Lemma vrf_alloc (Q : post ptr) i :
   (forall x, valid (x :-> v \+ i) -> Q (Val x) (x :-> v \+ i)) ->
   vrf i alloc Q.
 Proof.
 move=>H Vi /=.
-exists I=>_ _ [_][x][-> -> <- Hx Hx2].
+exists I=>_ _ [x][-> -> Hx Hx2].
 by apply: H; rewrite validPtUn Hx Vi.
 Qed.
 
@@ -834,33 +748,27 @@ End Allocation.
 Section BlockAllocation.
 Variables (A : Type) (v : A) (n : nat).
 
-Definition allocb_pre : pre := PredT.
+Definition allocb_pre : pre := top.
 
 Definition allocb_prog : prog allocb_pre ptr :=
-  fun p y m =>
-    exists i l, [/\ y = Val l, m = updi l (nseq n v) \+ i,
-                    i \In id_val p & valid m].
+  fun i _ _ y m =>
+    exists l, [/\ y = Val l, m = updi l (nseq n v) \+ i & valid m].
 
-Lemma allocb_coherent : coherent allocb_prog.
-Proof.
-move=>p x m; split.
-- by case=>i [l][{x}-> {m}-> Hi V]; exists i, Hi, i, l.
-by case=>i [Hi][_][l][{x}-> {m}-> <- V]; exists i, l.
-Qed.
+Lemma allocb_sfmono : safe_mono allocb_pre.
+Proof. by []. Qed.
 
 Lemma allocb_dstrict : def_strict allocb_prog.
-Proof. by case=>p H y[m][/= l][]. Qed.
+Proof. by move=>i [] Vi y [l][]. Qed.
 
 Lemma allocb_frame : frameable allocb_prog.
 Proof.
-move=>i j [[] Vi] Vij.
-exists I=>y m [_][l][/= {y}-> {m}-> <- V].
-exists (updi l (nseq n v) \+ i); rewrite -joinA; do!split=>//.
-exists i, l; do!split=>//.
+move=>i j [] Vij [] _ _ [l][->-> V].
+exists (updi l (nseq n v) \+ i); rewrite -joinA; split=>//.
+exists l; split=>//.
 by rewrite joinA in V; apply: (validL V).
 Qed.
 
-Definition allocb := Prog allocb_coherent allocb_dstrict allocb_frame.
+Definition allocb := Prog allocb_sfmono allocb_dstrict allocb_frame.
 
 Lemma vrf_allocb (Q : post ptr) i :
         (forall x, valid (updi x (nseq n v) \+ i) ->
@@ -868,7 +776,7 @@ Lemma vrf_allocb (Q : post ptr) i :
         vrf i allocb Q.
 Proof.
 move=>H Vi /=.
-exists I=>y m [_][l][/= {y}-> {m}-> <- V].
+exists I=>_ _ [l][->-> V].
 by apply: H.
 Qed.
 
@@ -881,37 +789,34 @@ Variable x : ptr.
 Definition dealloc_pre : pre :=
   fun i => x \in dom i.
 
-Definition dealloc_prog (p : ideald dealloc_pre) (y : ans unit) m :=
-  exists i, [/\ y = Val tt, m = free i x, i \In id_val p & x \in dom i].
+Definition dealloc_prog : prog dealloc_pre unit :=
+  fun i _ _ y m =>
+    [/\ y = Val tt, m = free i x & x \in dom i].
 
-Lemma dealloc_coherent : coherent dealloc_prog.
+Lemma dealloc_sfmono : safe_mono dealloc_pre.
 Proof.
-move=>p y m; split.
-- by case=>i [{y}-> {m}-> Hi Hx]; exists i, Hi, i.
-by case=>i [Hi][_][{y}-> {m}-> <- Hx]; exists i.
+move=>i j; rewrite /dealloc_pre -!toPredE /= => Hx Vij.
+by rewrite domUn inE Vij Hx.
 Qed.
 
 Lemma dealloc_dstrict : def_strict dealloc_prog.
 Proof.
-case=>p H _ [i][/= _ Hu Hi _]; case/H: Hi=> _ {H}Vi.
-suff {Hu}: valid (free i x) by rewrite -Hu.
+move=>i _ Vi _ [_ E _].
+suff {E}: valid (free i x) by rewrite -E.
 by rewrite validF.
 Qed.
 
 Lemma dealloc_frame : frameable dealloc_prog.
 Proof.
-move=>i j [Hi Vi] Vij.
-have J: i \+ j \In dealloc_pre.
-- by rewrite /dealloc_pre -toPredE /= domUn inE Vij Hi.
-exists J=>_ _ [_][-> -> <- Hx].
-exists (free i x); do!split.
-- by apply/freeUnR/dom_inNL/Hi.
-- by apply: validFUn.
-by exists i.
+move=>i j Hx Vij Hx' _ _ [->-> _].
+exists (free i x); split=>//;
+rewrite /dealloc_pre -!toPredE /= in Hx Hx'.
+- by apply/freeUnR/dom_inNL/Hx.
+by apply: validFUn.
 Qed.
 
 Definition dealloc :=
-  Prog dealloc_coherent dealloc_dstrict dealloc_frame.
+  Prog dealloc_sfmono dealloc_dstrict dealloc_frame.
 
 Lemma vrf_dealloc (Q : post unit) B (v : B) j:
         (x \notin dom j -> valid j -> Q (Val tt) j) ->
@@ -920,7 +825,7 @@ Proof.
 move=>H Vi /=.
 have J: x :-> v \+ j \In dealloc_pre.
 - by rewrite /dealloc_pre -toPredE /= domPtUnE.
-exists J=>_ _ [_][-> -> <- Hx].
+exists J=>_ _ [->-> Hx].
 rewrite freePtUn //; apply: H; last by exact: (validR Vi).
 by move: Hx; rewrite domPtUnE validPtUn; case/and3P.
 Qed.
